Support the POSIX empty capture

RegexPosix/POSIX.lean
@@ -22,14 +22,27 @@ inductive POSIX : {r : Regex α} → Parse r → Prop
     POSIX p₂ →
     ¬(∃ s₃ s₄, s₃ ≠ [] ∧ s₃ ++ s₄ = p₂.flat ∧ r₁.Matches (p₁.flat ++ s₃) ∧ r₂.Matches s₄) →
     POSIX (p₁.seq p₂)
-  | star_nil :
-    POSIX star_nil
+  | star_nil {r : Regex α} :
+    ¬r.nullable →
+    @POSIX r.star star_nil
+  | star_nil_null {r : Regex α} {p : Parse r} :
+    r.nullable →
+    POSIX p →
+    p.flat = [] →
+    POSIX (p.star_cons star_nil)
   | stars {r : Regex α} {p : Parse r} {ps : Parse (star r)} :
     POSIX p →
     POSIX ps →
     p.flat ≠ [] →
+    ps.flat ≠ [] →
     ¬(∃ s₃ s₄, s₃ ≠ [] ∧ s₃ ++ s₄ = ps.flat ∧ r.Matches (p.flat ++ s₃) ∧ (star r).Matches s₄) →
     POSIX (p.star_cons ps)
+  | stars_tail_empty {r : Regex α} {p : Parse r} {ps : Parse (star r)} :
+    POSIX p →
+    POSIX ps →
+    p.flat ≠ [] →
+    ps.flat = [] →
+    POSIX (p.star_cons star_nil)
 
 theorem POSIX.matches {r : Regex α} {p : Parse r} : POSIX p → r.Matches p.flat :=
   fun _ => p.matches
@@ -93,20 +106,49 @@ theorem POSIX.unique {r : Regex α} {p₁ p₂ : Parse r} (hp : p₁.flat = p₂
       simp at hp
       have hv' := longest_split_unique hp h₁₁.matches h₁₂.matches h₂₁.matches h₂₂.matches hs₁ hs₂
       rw [ih₁ hv'.left h₂₁, ih₂ hv'.right h₂₂]
-  | star_nil =>
+  | star_nil hn =>
     cases h₂ with
     | star_nil => rfl
+    | star_nil_null => contradiction
     | stars _ _ hp' =>
       simp at hp
       exact absurd hp.left hp'
-  | stars h₁₁ h₁₂ hp₁ hs₁ ih₁ ih₂ =>
+    | stars_tail_empty =>
+      simp at hp
+      contradiction
+  | star_nil_null hn hp₁ hp₁_flat ih =>
+    cases h₂ with
+    | star_nil => contradiction
+    | star_nil_null _ hp₂ =>
+      simp at hp
+      simp
+      exact ih hp hp₂
+    | stars => simp_all
+    | stars_tail_empty => simp_all
+  | stars h₁₁ h₁₂ hp₁ hp₂ hs₁ ih₁ ih₂ =>
     cases h₂ with
     | star_nil =>
       simp at hp
       exact absurd hp.left hp₁
-    | stars h₂₁ h₂₂ hp₂ hs₂ =>
+    | star_nil_null => simp_all
+    | stars h₂₁ h₂₂ hp₂ _ hs₂ =>
       simp at hp
       have hv' := longest_split_unique hp h₁₁.matches h₁₂.matches h₂₁.matches h₂₂.matches hs₁ hs₂
       have ih₂ := ih₂ hv'.right h₂₂
       simp at ih₂
       rw [ih₁ hv'.left h₂₁, ih₂]
+    | stars_tail_empty h₂₁ h₂₂ hp₂₁ hp₂₂ =>
+      simp only [flat] at hp
+      have hk := longest_split_unique hp h₁₁.matches h₁₂.matches h₂₁.matches (hp₂₂ ▸ h₂₂.matches) hs₁ (by simp)
+      simp_all
+  | stars_tail_empty h₁₁ h₁₂ hp₁₁ hp₁₂ ih₁ ih₂ =>
+    cases h₂ with
+    | star_nil => simp_all
+    | star_nil_null => simp_all
+    | stars h₂₁ h₂₂ hp₂₁ hp₂₂ hs =>
+      simp only [flat] at hp
+      have hk := longest_split_unique hp.symm h₂₁.matches h₂₂.matches h₁₁.matches (hp₁₂ ▸ h₁₂.matches) hs (by simp)
+      simp_all
+    | stars_tail_empty h₂₁ h₂₂ hp₂₁ hp₂₂ =>
+      simp at hp
+      simp [ih₁ hp h₂₁]
